adjust the binary log rel resources

src/OSum/binary_logrel.v
@@ -1,67 +1,44 @@
-From stdpp Require Import base gmap.
+From stdpp Require Import base gmap coPset tactics proof_irrel.
 
-From iris.base_logic Require Import invariants iprop upred saved_prop.
-From iris.base_logic.lib Require Import gset_bij .
-From iris.algebra Require Import gset_bij excl gmap.
+From iris.base_logic Require Import invariants iprop upred saved_prop gen_heap.
+From iris.base_logic.lib Require Import ghost_map gset_bij.
+From iris.algebra Require Import cofe_solver gset gmap_view excl gset_bij.
 From iris.proofmode Require Import proofmode.
 From iris.program_logic Require Import weakestpre.
 Require Import Autosubst.Autosubst.
 
-From Equations Require Import Equations.
+From MyProject.src.OSum Require Export OSum persistent_pred wp_rules binary_rules.
 
-From MyProject.src.OSum Require Export OSum persistent_pred wp_rules.
+Definition logN : namespace := nroot .@ "logN".
 
-Definition specN := nroot .@ "spec".
-
-
-
-Definition D `{Σ : gFunctors}:= persistent_pred (val * val) (iProp Σ).
-
-(* need to enhance state.. *)
-Class logrelSig  Σ := Resources {
-    invariants : invGS Σ;
+Class RelationResources Σ := RelRes{
     predicates :: savedPredG Σ (val * val) ;
-    names :: gset_bijG Σ loc loc ;
-    name_set : gname
-}.
-Check rtc.
-Check erased_step. 
-Locate erased_step.
-Check gset_bijR.
-
-
-Definition combine (l1 l2 : list loc) : gset (loc * loc) := 
-    list_to_set (zip l1 l2).
-
-Definition spec_thread : cmra := exclR exprO.
-Definition configRA : cmra := prodR spec_thread (gset_bijR loc loc).
-
-Definition as_thread (e : expr) : spec_thread := Excl e.
-
-Class configSpec Σ := CS { 
-    config_in :: inG Σ configRA ; 
-    spec_predicates :: savedPredG Σ (val * val) ;
-    config_name : gname
+    rel_bijection :: gset_bijG Σ (loc * loc) loc ;
+    name_bijection :: gset_bijG Σ loc loc;
+    sets :: inG Σ (authR (gsetUR loc))
 }.
 
-Section definitionsS.
-    Context `{configSpec Σ, invGS Σ}.
-    Definition spec_inv (ρ : cfg OSum_lang) : iProp Σ := 
-        (∃ e s s', own config_name (Excl e , ●V (combine s s'))
-                    ∗ [∗ list] l' ∈ s', (∃ (P : D), saved_pred_own l' (DfracDiscarded) P)
-                    ∗ ⌜rtc erased_step ρ ([e],s)⌝)%I.
+Class relStore  Σ  := RelStore {
+    resources :: RelationResources Σ ; 
+    rel_bij : gname ;
+    name_bij : gname; 
+    name_set : gname;
+}.
 
-    Definition spec_ctx : iProp Σ :=
-        (∃ ρ, inv specN (spec_inv ρ))%I.
-    
-End definitionsS.
+Class logrelSig Σ := LogRelSig {
+    invariants : invGS Σ;
+    store :: relStore  Σ ;
+}.
 
+Definition D `{ts : !relStore Σ}:= persistent_pred (val * val) (iProp Σ).
 
+Definition state_interp  `{ts : !relStore Σ}(s : list loc) : iProp Σ :=
+    own name_set (● (list_to_set s)).
 
-Definition state_interp `{logrelSig Σ} (s : list loc) : iProp Σ :=
-    ∃ (s' : list loc ) , 
-            gset_bij_own_auth name_set (DfracOwn 1) (combine s s')  ∗
-            [∗ list] l' ∈ s', (∃ (P : D), saved_pred_own l' (DfracDiscarded) P).
+Definition state_elem `{ts : !relStore Σ} (l : loc) : iProp Σ :=
+    own name_set (◯ (singleton l)).
+
+Notation "l ∈i" := (state_elem l) (at level 20) : bi_scope.
 
 
 Global Instance OSum_irisGS `{logrelSig Σ} : irisGS OSum_lang Σ := {
@@ -71,3 +48,205 @@ Global Instance OSum_irisGS `{logrelSig Σ} : irisGS OSum_lang Σ := {
     fork_post _ := True%I;
     state_interp_mono _ _ _ _ := fupd_intro _ _
 }.
+
+Section binary_logrel.
+    Context`{logrelSig Σ, configSpec Σ}.
+
+    Definition VRel := listO D -n> D.
+
+    Program Definition pointsto_def (l l' : loc) : D -n> iPropO Σ  :=
+    λne R, (∃ (l'' : loc), 
+            gset_bij_own_elem name_bij l l'  ∗
+            gset_bij_own_elem rel_bij (l , l') l''  ∗ 
+            saved_pred_own l'' DfracDiscarded R)%I.
+    Next Obligation. Admitted.
+
+    Notation "l @ l' ↦□ R" := (pointsto_def l l' R)
+    (at level 20,  format "l @ l' ↦□ R") : bi_scope.
+
+    Instance mypointsto_persist (l l': loc)  (R : D) : Persistent (l @ l' ↦□ R).
+    apply _. Qed.
+
+    Definition interp_expr (τi :  VRel) (Δ : listO D) (ee : expr * expr) : iProp Σ := 
+    (∀ K, ⤇ fill K (ee.2) -∗
+        WP ee.1 {{ v, ∃ v', ⤇ fill K (of_val v') ∧ τi Δ (v, v') }})%I.
+
+    Global Instance interp_expr_ne n :
+        Proper (dist n ==> dist n ==> (=) ==> dist n) interp_expr.
+    Proof. unfold interp_expr; solve_proper. Qed.
+
+    
+    Program Definition interp_TVar (v : var) : VRel := 
+        λne rho, PersPred (default (inhabitant : persistent_pred _ _) (rho !! v)).
+    Solve Obligations with repeat intros ?; simpl; solve_proper.
+
+    Program Definition interp_TUnit : VRel := 
+    λne rho, PersPred(fun w => ⌜w.1 = UnitV /\ w.2 = UnitV⌝%I).
+
+    Definition interp_TInt : VRel := 
+    λne rho, PersPred(fun w =>(∃ (z : Z), ⌜w.1 = IntV z /\ w.2 = IntV z⌝))%I.
+
+    Definition interp_TBool : VRel := 
+    λne rho, PersPred(fun w => (∃ (b : bool), ⌜w.1 = BoolV b /\ w.2 = BoolV b⌝))%I.
+
+    Program Definition interp_TProd (interp1 interp2 : VRel) : VRel := 
+        λne rho, PersPred(fun w => (∃ vv1 vv2 , 
+            ⌜w = (PairV vv1.1 vv2.1 ,PairV vv1.2 vv2.2)⌝  ∧ 
+            interp1 rho vv1  ∧ 
+            interp2 rho vv2))%I.  
+    Solve Obligations with solve_proper.
+
+    Definition case_inv (l l' : loc)(R : D): iProp Σ := 
+        state_elem l ∧
+        spec_state_elem l' ∧ 
+        l @ l' ↦□ R.
+
+    Program Definition interp_TCase (interp : VRel) : VRel := 
+        λne rho, PersPred(fun w => 
+            ∃ (l l' : loc), 
+                ⌜w = (CaseV l , CaseV l')⌝ ∧
+                (case_inv l l' (interp rho)))%I.
+                (* can I get away with not using inv here? *)
+(*                 inv (logN .@ (l,l')) (case_inv l l' (interp rho)))%I.
+ *)    Next Obligation. Admitted.
+
+    Definition interp_TOSum : VRel := 
+        λne rho, PersPred(fun w => 
+            ∃ (l l' : loc)(v1 v2 : val)(R : D),
+                ⌜w = (InjV (CaseV l) v1 , InjV (CaseV l') v2)⌝ ∧
+                l @ l' ↦□ R ∧
+                R (v1 ,v2))%I.
+
+    Program Definition interp_TArrow (interp1 interp2 : VRel) : VRel :=
+        λne Δ,
+        PersPred
+        (λ ww, □ ∀ vv, interp1 Δ vv →
+                        interp_expr
+                            interp2 Δ (App (of_val (ww.1)) (of_val (vv.1)),
+                                        App (of_val (ww.2)) (of_val (vv.2))))%I.
+    Solve Obligations with solve_proper.
+      
+    Program Definition interp_TForall (interp : VRel) : VRel :=
+        λne Δ, PersPred(fun ww =>
+            □ ∀ τi,
+                interp_expr
+                interp (τi :: Δ) (TApp (of_val (ww.1)), TApp (of_val (ww.2))))%I.
+    Solve Obligations with solve_proper.
+
+    Program Definition interp_TExist (interp : VRel) : VRel :=
+        λne Δ,PersPred
+            (λ ww, ∃ (τi : D) vv, ⌜ww = (PackV vv.1, PackV vv.2)⌝ ∗
+               interp (τi :: Δ) vv)%I.
+    Solve Obligations with repeat intros ?; simpl; solve_proper.
+
+    Fixpoint interp (τ : type) : VRel :=
+        match τ return _ with
+            | TUnit => interp_TUnit
+            | TInt => interp_TInt
+            | TBool => interp_TBool
+            | TProd τ1 τ2 => interp_TProd (interp τ1) (interp τ2)
+            | TArrow τ1 τ2 => interp_TArrow (interp τ1) (interp τ2)
+            | TVar x => interp_TVar x
+            | TForall τ' => interp_TForall (interp τ')
+            | TExist τ' => interp_TExist (interp τ')
+            | TOSum => interp_TOSum
+            | TCase t => interp_TCase (interp t)
+        end.
+    Notation "⟦ τ ⟧" := (interp τ).
+
+    Notation "⟦ τ ⟧ₑ" := (interp_expr (interp τ)).
+
+
+    Definition interp_env (Γ : list type)
+    (Δ : list D) (vs : list (val * val)) : iProp Σ :=
+    (⌜length Γ = length vs⌝ ∗ [∗] zip_with (λ τ, ⟦ τ ⟧ Δ) Γ vs)%I.
+    Notation "⟦ Γ ⟧*" := (interp_env Γ).
+
+    Global Instance interp_env_base_persistent Δ Γ vs :
+    TCForall Persistent (zip_with (λ τ, ⟦ τ ⟧ Δ) Γ vs).
+    Proof. revert vs; induction Γ => vs; destruct vs; constructor; apply _. Qed.
+    Global Instance interp_env_persistent Γ Δ vs : Persistent (⟦ Γ ⟧* Δ vs) := _.
+
+
+    Lemma interp_env_nil Δ : ⊢ ⟦ [] ⟧* Δ [].
+    Proof. iSplit; simpl; auto. Qed.
+
+    Import uPred.
+    Lemma interp_env_cons Δ Γ vvs τ vv :
+        ⟦ τ :: Γ ⟧* Δ (vv :: vvs) ⊣⊢ ⟦ τ ⟧ Δ vv ∗ ⟦ Γ ⟧* Δ vvs.
+    Proof.
+        rewrite /interp_env /= (assoc _ (⟦ _ ⟧ _ _)) -(comm _ ⌜(_ = _)⌝%I) -assoc.
+        by apply sep_proper; [apply pure_proper; lia|].
+    Qed.
+
+
+    Lemma interp_env_length Δ Γ vs : ⟦ Γ ⟧* Δ vs ⊢ ⌜length Γ = length vs⌝.
+    Proof. by iIntros "[% ?]". Qed.
+
+    Lemma interp_env_Some_l Δ Γ vs x τ :
+        Γ !! x = Some τ → ⟦ Γ ⟧* Δ vs ⊢ ∃ v, ⌜vs !! x = Some v⌝ ∧ ⟦ τ ⟧ Δ v.
+    Proof.
+        iIntros (?) "[Hlen HΓ]"; iDestruct "Hlen" as %Hlen.
+        destruct (lookup_lt_is_Some_2 vs x) as [v Hv].
+        { by rewrite -Hlen; apply lookup_lt_Some with τ. }
+        iExists v; iSplit; first done. iApply (big_sepL_elem_of with "HΓ").
+        apply elem_of_list_lookup_2 with x.
+        rewrite lookup_zip_with; by simplify_option_eq.
+    Qed.
+
+    (*  need to fix this proof *)
+    Lemma interp_weaken Δ1 Π Δ2 τ :
+        ⟦ τ.[upn (length Δ1) (ren (+ length Π))] ⟧ (Δ1 ++ Π ++ Δ2)
+        ≡ ⟦ τ ⟧ (Δ1 ++ Δ2).
+    Proof.
+        revert Δ1 Π Δ2. induction τ=> Δ1 Π Δ2; simpl; auto; intros ?; simpl.
+        - by repeat (f_equiv; try match goal with IH : ∀ _, _ |- _ => by apply IH end).
+        - 
+        Admitted.
+    (*     - by repeat (f_equiv; try match goal with IH : ∀ _, _ |- _ => by apply IH end).
+        - f_equiv.
+        apply fixpoint_proper=> τi w /=.
+        by repeat (f_equiv; try match goal with IH : ∀ _, _ |- _ => by apply (IH (_ :: _)) end).
+        - rewrite iter_up; destruct lt_dec as [Hl | Hl]; simpl.
+        { by rewrite !lookup_app_l. }
+        rewrite !lookup_app_r; [|lia ..]; do 3 f_equiv; lia.
+        - by repeat (f_equiv; try match goal with IH : ∀ _, _ |- _ => by apply (IH (_ :: _)) end).
+        - by repeat (f_equiv; try match goal with IH : ∀ _, _ |- _ => by apply (IH (_ :: _)) end).
+        - by repeat (f_equiv; try match goal with IH : ∀ _, _ |- _ => by apply IH end).
+    Qed. *)
+
+    (* need to fix this proof  *)
+    Lemma interp_subst_up Δ1 Δ2 τ τ' :
+        ⟦ τ ⟧ (Δ1 ++ interp τ' Δ2 :: Δ2)
+        ≡ ⟦ τ.[upn (length Δ1) (τ' .: ids)] ⟧ (Δ1 ++ Δ2).
+    Proof.
+        revert Δ1 Δ2; induction τ=> Δ1 Δ2; simpl; auto; intros ?; simpl.
+        - by repeat (f_equiv; try match goal with IH : ∀ _, _ |- _ => by apply IH end).
+        - 
+        Admitted. (* by repeat (f_equiv; try match goal with IH : ∀ _, _ |- _ => by apply IH end).
+        - f_equiv.
+        apply fixpoint_proper=> τi w /=.
+        by repeat (f_equiv; try match goal with IH : ∀ _, _ |- _ => by apply (IH (_ :: _)) end).
+        - match goal with |- context [_ !! ?x] => rename x into idx end.
+        rewrite iter_up; destruct lt_dec as [Hl | Hl]; simpl.
+        { by rewrite !lookup_app_l. }
+        rewrite !lookup_app_r; [|lia ..].
+        case EQ: (idx - length Δ1) => [|n]; simpl.
+        { symmetry. asimpl. apply (interp_weaken [] Δ1 Δ2 τ'). }
+        rewrite !lookup_app_r; [|lia ..]. do 3 f_equiv. lia.
+        - by repeat (f_equiv; try match goal with IH : ∀ _, _ |- _ => by apply (IH (_ :: _)) end).
+        - by repeat (f_equiv; try match goal with IH : ∀ _, _ |- _ => by apply (IH (_ :: _)) end).
+        - by repeat (f_equiv; try match goal with IH : ∀ _, _ |- _ => by apply IH end).
+    Qed. *)
+
+    (* fix this  *)
+    Lemma interp_subst Δ2 τ τ' v : ⟦ τ ⟧ (⟦ τ' ⟧ Δ2 :: Δ2) v ≡ ⟦ τ.[τ'/] ⟧ Δ2 v.
+    Admitted.
+
+
+End binary_logrel.
+
+Global Typeclasses Opaque interp_env.
+Notation "⟦ τ ⟧" := (interp τ).
+Notation "⟦ τ ⟧ₑ" := (interp_expr (interp τ)).
+Notation "⟦ Γ ⟧*" := (interp_env Γ).
