src/OSum/binary_fundamental.v
@@ -1,0 +1,418 @@
+From stdpp Require Import base gmap coPset tactics proof_irrel sets.
+
+From iris.base_logic Require Import invariants iprop upred saved_prop gen_heap.
+From iris.base_logic.lib Require Import ghost_map gset_bij.
+From iris.algebra Require Import cofe_solver gset gmap_view excl gset_bij.
+From iris.proofmode Require Import proofmode.
+From iris.program_logic Require Import weakestpre ectx_lifting ectx_language.
+Require Import Autosubst.Autosubst.
+
+
+From MyProject.src.OSum Require Export OSum binary_logrel binary_rules.
+
+Fixpoint env_subst (vs : list val) : var → expr :=
+match vs with
+| [] => ids
+| v :: vs' => (of_val v) .: env_subst vs'
+end.
+
+Section bin_log_def.
+    Context `{logrelSig Σ, configSpec Σ}.
+
+    Check interp_expr.
+    Check interp.
+    Check interp_env.
+    Definition bin_log_related (Γ : list type)(e e' : expr)(t : type) : iProp Σ := 
+        (□ ∀ rho ws, 
+            spec_ctx ∧ ⟦ Γ ⟧* rho ws -∗  
+            ⟦ t ⟧ₑ rho (e.[env_subst (ws.*1)], e'.[env_subst (ws.*2)]))%I.
+
+    
+    Global Instance: ∀ Γ e e' τ, Persistent (bin_log_related Γ e e' τ).
+    Proof. rewrite/bin_log_related /=. apply _. Qed.
+      
+End bin_log_def.
+      
+Notation "Γ ⊨ e '≤log≤' e' : τ" :=
+    (bin_log_related Γ e e' τ) (at level 74, e, e', τ at next level).
+      
+Section fundamental.
+    Context `{logrelSig Σ, configSpec Σ}.
+
+    Lemma bin_log_rel_unit Γ : ⊢ Γ ⊨ Unit ≤log≤ Unit : TUnit.
+    Proof.
+        (* unpack binary logical relation definition *)
+        iIntros (rho ws).
+        iModIntro.
+        iIntros "(#Hs & #HGam)".
+        (* unpack interpretation of expressions *)
+        unfold interp_expr; asimpl.
+        iIntros (K) "Hspec". 
+        (* Unit is a value *)
+        iApply wp_value.
+        iExists UnitV.
+        iSplit.
+        - iApply "Hspec".
+        - done.
+    Qed.
+
+    Lemma bin_log_rel_bool Γ b : ⊢ Γ ⊨ Bool b ≤log≤ Bool b : TBool.
+    Proof.
+        iIntros (rho ws) "!#(#Hs & #Hgam)".
+        unfold interp_expr; asimpl.
+        iIntros (K) "Hspec".
+        iApply wp_value.
+        iExists (BoolV b).
+        iSplit.
+        - iApply "Hspec".
+        - iExists b. done.
+    Qed.
+        
+    Lemma bin_log_rel_int Γ n : ⊢ Γ ⊨ Int n ≤log≤ Int n : TInt.
+    Proof.
+        iIntros (rho ws) "!#(#Hs & #Hgam)".
+        unfold interp_expr; asimpl.
+        iIntros (k) "Hspec".
+        iApply wp_value.
+        iExists (IntV n).
+        iSplit.
+        - iApply "Hspec".
+        - iExists n. done.
+    Qed.
+
+    Lemma interp_expr_bind KK ee Δ τ τ' :
+    ⟦ τ ⟧ₑ Δ ee -∗
+    (∀ vv, ⟦ τ ⟧ Δ vv -∗ ⟦ τ' ⟧ₑ Δ (fill KK.1 (of_val vv.1), fill KK.2 (of_val vv.2))) -∗
+    ⟦ τ' ⟧ₑ Δ (fill KK.1 ee.1, fill KK.2 ee.2).
+  Proof.
+    iIntros "He HK" (Z) "Hj /=".
+    iSpecialize ("He" with "[Hj]"); first by rewrite -fill_app; iFrame.
+    iApply wp_bind.
+    iApply (wp_wand with "He").
+    iIntros (?); iDestruct 1 as (?) "[? #?]".
+    iApply ("HK" $! (_, _)); [done| rewrite /= fill_app //].
+  Qed.
+
+  Lemma interp_expr_bind' K K' e e' Δ τ τ' :
+    ⟦ τ ⟧ₑ Δ (e, e') -∗
+    (∀ vv, ⟦ τ ⟧ Δ vv -∗ ⟦ τ' ⟧ₑ Δ (fill K (of_val vv.1), fill K' (of_val vv.2))) -∗
+    ⟦ τ' ⟧ₑ Δ (fill K e, fill K' e').
+  Proof. iApply (interp_expr_bind (_, _) (_, _)). Qed.
+
+    Lemma interp_expr_val vv rho t : ⟦ t ⟧ rho vv -∗ ⟦ t ⟧ₑ rho (of_val vv.1, of_val vv.2).
+  Proof. destruct vv. iIntros "?" (?) "?". iApply wp_value. iExists _. iFrame. Qed.
+
+    Lemma bin_log_rel_pair Γ t1 t2 e1 e2 e3 e4 :
+        Γ ⊨ e1 ≤log≤ e2 : t1 -∗
+        Γ ⊨ e3 ≤log≤ e4 : t2 -∗
+        Γ ⊨ Pair e1 e3 ≤log≤ Pair e2 e4 : TProd t1 t2.
+    Proof.
+        (* assumptions *)
+        iIntros "#Hp1 #Hp2" (rho ws) "!#(#Hs & #Hgam)" .
+        iIntros (K) "Hspec". 
+        (* specialize Hp1 and Hp2 *)
+        iSpecialize ("Hp1" $! rho ws with "[# $Hs  $Hgam]").
+        iSpecialize ("Hp2" $! rho ws with "[# $Hs  $Hgam]").
+        (* reduce the pair to values 
+           first the left side *)
+        iApply (interp_expr_bind' [PairLCtx _] [PairLCtx _]).
+        1:{ iApply "Hp1". }
+        2:{ asimpl. iApply "Hspec". }
+        (* now the right side *)
+        iIntros ([v1 v2]) "#Hv12".
+        iApply (interp_expr_bind' [PairRCtx _] [PairRCtx _]).
+        { iApply "Hp2". }
+        iIntros ([v3 v4]) "#Hv34".
+        (* now we have a value *)
+        iApply (interp_expr_val (PairV _ _, PairV _ _)).
+        (* use the value interpretation of products *)
+        iExists (v1 , v2). iExists (v3 , v4). fold interp.
+        (* and we are done *)
+        repeat iSplit ; done.
+    Qed.
+
+    (* pick up to_of_val in eauto
+       usage in apply step_fst, see hypothesis *)
+    Local Hint Resolve to_of_val : core.
+
+    Lemma bin_log_rel_fst Γ t1 t2 p1 p2 : 
+        Γ ⊨ p1 ≤log≤ p2 : TProd t1 t2 -∗
+        Γ ⊨ Fst p1 ≤log≤ Fst p2 : t1.
+    Proof.
+        (* assumptions *)
+        iIntros "#Hp" (rho ws) "!#(#Hs & #Hgam)" .
+        iIntros (K) "Hspec". 
+        (* specialize Hp *)
+        iSpecialize ("Hp" $! rho ws with "[# $Hs $Hgam]").
+        (* use bind to get to fill FstCtx e*)
+        iApply (interp_expr_bind' [FstCtx] [FstCtx]).
+        { iApply "Hp". }
+        2:{ asimpl. iApply "Hspec". }
+        (* the main proof of the expr bind *)
+        iIntros ([v  v']) "#Hv".
+        (* break apart the hypothesis intepr (v ,v') *) 
+        iDestruct "Hv" as ([v1 v1'][v2 v2']) "#[%Heq [Hv1 Hv2]]" ;fold interp in * 
+        ;simpl in Heq; inversion Heq; subst; simpl. 
+        (* we have Fst (Pair _ _ ) which can step*)
+        (* first, take in the spec config *)
+        iIntros (K') "Hspec "; simpl.
+        (* now step *)
+        iApply wp_pure_step_later; try done.
+        iIntros "!> _".
+        (* take a specification step *)
+        iMod (step_fst with "[Hspec]") as "Hspec'" ; eauto .
+        iApply wp_value.
+        iExists v1'.
+        iSplit.
+        - iApply "Hspec'".
+        - iApply "Hv1".
+    Qed.
+
+    Lemma bin_log_rel_snd Γ t1 t2 p1 p2 : 
+        Γ ⊨ p1 ≤log≤ p2 : TProd t1 t2 -∗
+        Γ ⊨ Snd p1 ≤log≤ Snd p2 : t2.
+    Proof.
+        (* assumptions *)
+        iIntros "#Hp" (rho ws) "!#(#Hs & #Hgam)" .
+        iIntros (K) "Hspec". 
+        (* specialize Hp *)
+        iSpecialize ("Hp" $! rho ws with "[# $Hs $Hgam]").
+        (* use bind to get to fill SndCtx e*)
+        iApply (interp_expr_bind' [SndCtx] [SndCtx]).
+        { iApply "Hp". }
+        2:{ asimpl. iApply "Hspec". }
+        (* the main proof of the expr bind *)
+        iIntros ([v  v']) "#Hv".
+        (* break apart the hypothesis intepr (v ,v') *) 
+        iDestruct "Hv" as ([v1 v1'][v2 v2']) "#[%Heq [Hv1 Hv2]]" ;fold interp in * 
+        ;simpl in Heq; inversion Heq; subst; simpl. 
+        (* we have Snd (Pair _ _ ) which can step*)
+        (* first, take in the spec config *)
+        iIntros (K') "Hspec "; simpl.
+        (* now step *)
+        iApply wp_pure_step_later; try done.
+        iIntros "!> _".
+        (* take a specification step *)
+        Check step_snd.
+        iMod (step_snd with "[Hspec]") as "Hspec'" ; eauto .
+        iApply wp_value.
+        iExists v2'.
+        iSplit.
+        - iApply "Hspec'".
+        - iApply "Hv2".
+    Qed.
+
+    Lemma bin_log_rel_osum Γ t c1 c2 e1 e2 : 
+        Γ ⊨ c1 ≤log≤ c2 : TCase t -∗
+        Γ ⊨ e1 ≤log≤ e2 : t -∗
+        Γ ⊨ Inj c1 e1 ≤log≤ Inj c2 e2 : TOSum.
+    Proof.
+        (* assumptions *)
+        iIntros "#Hc #He" (rho ws) "!#(#Hs & #Hgam)" .
+        iIntros (K) "Hspec". 
+        (* specialize  *)
+        iSpecialize ("Hc" $! rho ws with "[# $Hs $Hgam]").
+        iSpecialize ("He" $! rho ws with "[# $Hs $Hgam]").
+        (* bind *)
+        iApply (interp_expr_bind' [InjLCtx _] [InjLCtx _]).
+        { iApply "Hc". }
+        2:{ iApply "Hspec". }
+        iIntros ([cv1 cv2]) "#Hcv".
+        iApply (interp_expr_bind' [InjRCtx _] [InjRCtx _]).
+        {iApply "He". }
+        iIntros ([ev1 ev2]) "#Hev".
+        (* we have values *)
+        iApply (interp_expr_val (InjV _ _, InjV _ _)).
+        (* break apart our assumptions on the pair or cases and pair of e:t  *)
+        iDestruct "Hcv" as "[%l [%l' [%Heqcase Hinv]]]"; fold interp in *; inversion Heqcase; subst.
+        iDestruct "Hinv" as "[limp [lspec point]]".
+        iExists l , l' , ev1 , ev2, (interp t rho).
+        repeat iSplit ; try done.
+    Qed.
+
+(*         (* break apart out assumptions on the pair or cases and pair of e:t  *)
+        iDestruct "Hcv" as "[%l [%l' [%Heqcase Hinv]]]"; fold interp in * ;inversion Heqcase; subst.
+        iIntros (K') "Hspec".
+        iInv "Hinv" as "foo". (* if we use inv, can use iInv when the goal is a Wp *)
+        {
+            apply ectx_language_atomic; simpl.
+            2:{ red. intros. inversion H1. }
+            simpl. red. intros. apply prim_base_irreducible.
+             red. intros. unfold not. intros.  
+        }
+ *)
+
+    Lemma bin_log_rel_caseof Γ e1 e2 e3 e4 e1' e2' e3' e4' t1 t2: 
+        Γ ⊨ e1 ≤log≤ e1' : TOSum -∗
+        Γ ⊨ e2 ≤log≤ e2' : TCase t1 -∗
+        t1 :: Γ ⊨ e3 ≤log≤ e3' : t2 -∗
+        Γ ⊨ e4 ≤log≤ e4' : t2 -∗
+        Γ ⊨ CaseOf e1 e2 e3 e4 ≤log≤ CaseOf e1' e2' e3' e4' : t2.
+    Proof.
+        (* assumptions *)
+        iIntros "#Ho #Hc #Htru #Hfls" (rho ws) "!#(#Hs & #Hgam)" .
+        iIntros (K) "Hspec". 
+        (* specialize  *)
+        iSpecialize ("Ho" $! rho ws with "[# $Hs $Hgam]").
+        iSpecialize ("Hc" $! rho ws with "[# $Hs $Hgam]").
+        iSpecialize ("Hfls" $! rho ws with "[# $Hs $Hgam]").
+        (* reduce *)
+        iApply (interp_expr_bind' [CaseOfCtxOSUM _ _ _] [CaseOfCtxOSUM _ _ _]).
+        { iApply "Ho". }
+        2:{ iApply "Hspec". } 
+        iIntros ([ov1 ov2]) "#Hov".
+        iApply (interp_expr_bind' [CaseOfCtxInj _ _ _] [CaseOfCtxInj _ _ _]).
+        { iApply "Hc". } 
+        iIntros ([cv1 cv2]) "#Hcv".
+        (* use the value relation data for osum *)
+        iDestruct "Hov" as "[%l1 [%l1' [%ov1' [%ov2' [%R [%Heq [[%l3 [nbij1 [rbij1 pred1]]] Rel]]]]]]]".
+        inversion Heq. subst. 
+        (* use the value relation data for case *)
+        iDestruct "Hcv" as "[%l2 [%l2' [%Hceq Cinv]]]". fold interp in *.
+        inversion Hceq. subst.
+        (* destruct the case invariant *)
+        iDestruct "Cinv" as "[#l2in [#l2'in [%l3' [nbij2 [rbij2 pred2]]]]]".
+
+    
+        iIntros (K') "Hspec'".
+        simpl.
+
+        destruct (decide (l1 = l2)) as [|Hneq]. subst.
+        {
+            iPoseProof (gset_bij_own_elem_agree with "nbij1 nbij2") as "%foo".
+            destruct foo.
+            pose proof (H1 (eq_refl l2)). subst.
+            iPoseProof (gset_bij_own_elem_agree with "rbij1 rbij2") as "%bar".
+            destruct bar.
+            pose proof (H3 (eq_refl _)). subst.
+            iPoseProof (@saved_pred_agree _ _ _ _ _ _  _ _ (ov1' , ov2') with "pred1 pred2") as "baz".
+            iMod (step_caseOf_true with "[Hspec']") as "yosh".
+            3:{
+                iSplit. - iApply "Hs". -iApply "Hspec'".
+            }
+            {
+                apply to_of_val.
+            }
+            { eauto. }
+            iApply wp_pure_step_later; try done.
+            iIntros "!> _".
+            asimpl.
+            iSpecialize ("Htru" $! rho ((ov1' , ov2') :: ws)).
+            iAssert (⟦ t1 :: Γ ⟧* rho ((ov1', ov2') :: ws))%I as "Hext".
+            - iApply interp_env_cons.
+            iSplit.
+            + iRewrite -"baz". iApply "Rel".
+            + iApply "Hgam".
+            - iSpecialize ("Htru"  with "[Hs Hext]").
+            + iSplit. iApply "Hs". iApply "Hext".
+            + asimpl.
+            iApply "Htru". simpl.
+            iApply "yosh".
+        }
+        iPoseProof (gset_bij_own_elem_agree with "nbij1 nbij2") as "%foo".
+        assert (l1' <> l2').
+        {
+            destruct foo. unfold not. intros. auto.
+        }
+        iMod (step_caseOf_false with "[Hspec']") as "yosh".
+        4: {
+            iSplit. - done.
+            - iApply "Hspec'".
+        }
+        { apply to_of_val. } done. done.
+        iApply wp_pure_step_later.
+        { apply wp_case_nomatch. - red. exists ov1'. done. - done. }
+        done.
+        iIntros "!> _".
+        iApply "Hfls".
+        iApply "yosh".
+    Qed.
+
+    Check New.
+    (*  In the unary version.. I have the authoritative element of the 
+    bijection given from the state interpretation.. 
+    
+    Which .. seems fine in the unary case
+    but in the binary case, the state interpretation including the 
+    authoritative element of the bijection is positing
+    the existence of a separate executeion whos program state is 
+    in bijection with the currently running program..
+
+    Maybe this is a misuse of the state interpretation and it should
+    instead be an invariant on the locations
+    *)
+    Lemma wp_new t  : 
+        ⊢ WP (New t) {{ v, ∃ l , ⌜v = CaseV l⌝ ∗ own name_set (◯ (singleton l))}}.
+    Proof.
+        iApply wp_lift_atomic_base_step_no_fork; auto;  simpl.
+        iIntros (s1 _ k1  _ _) "ownS". 
+                    (* get access to the state interpretation *)
+        unfold binary_logrel.state_interp; simpl; unfold state_interp.
+        (* handle the fact that New is reducible first *)
+        iModIntro. iSplit.
+        - iPureIntro; unfold base_reducible; repeat eexists; eapply NewS.
+        (* only obligation is that we need to be able to summon a fresh name *)
+    (*         exact (is_fresh s1).
+    *)      - (* now we need to handle the state update, 
+            first bring variables into scope  *)
+        iModIntro. iIntros (e2 s2 efs baseStep) "lc".
+        (* inversion on the base step *)
+        inversion baseStep. subst ; simpl.
+        iApply fupd_frame_l.
+        iSplit; try done.
+        iApply fupd_frame_r.
+    Admitted.
+ (*        iSplit.
+        2:{ iExists (fresh s1). done. }
+        iMod (own_update with "[ownS]") as "goal".
+        2:{ iApply "ownS". }
+        { 
+            red.
+        } 
+        Check auth_update.
+        iApply own_update.
+        Check own_update. *)
+  
+    
+    Lemma bin_log_rel_new Γ t : 
+        ⊢ Γ ⊨ New t ≤log≤ New t : TCase t.
+    Proof.
+        iIntros (rho ws) "!#(#Hs & #Hgam)".
+        iIntros (K) "Hspec".
+        asimpl.
+        iApply wp_wand.
+        iApply wp_new.
+        iIntros (v) "[%l [%leq ownl]]". subst.
+        
+
+        unfold case_inv. unfold pointsto_def. simpl. subst.
+    Admitted.
+
+
+    Theorem binary_fundamental Γ e t : 
+        Γ ⊢ₜ e : t → ⊢ Γ ⊨ e ≤log≤ e : t.
+    Proof.
+        intros typ.
+        induction typ.
+        - admit.
+        - iApply bin_log_rel_unit.
+        - iApply bin_log_rel_int.
+        - iApply bin_log_rel_bool.
+        - admit.
+        - admit.
+        - iApply bin_log_rel_pair ; done.
+        - iApply bin_log_rel_fst; done.
+        - iApply bin_log_rel_snd; done.
+        - iApply bin_log_rel_osum ; done.
+        - iApply bin_log_rel_caseof; done.
+        - iApply bin_log_rel_new.
+        - admit.
+        - admit.
+        - admit.
+        - admit.
+        - admit.
+        - admit.
+        - admit.
+        - admit.
+    Admitted.
+End fundamental.
