src/OSum/binary_rules.v
@@ -1,0 +1,242 @@
+From stdpp Require Import base gmap.
+
+From iris.base_logic Require Import invariants iprop upred saved_prop.
+From iris.base_logic.lib Require Import gset_bij .
+From iris.algebra Require Import gset_bij excl gmap gset cmra.
+From iris.proofmode Require Import proofmode.
+From iris.program_logic Require Import weakestpre.
+Require Import Autosubst.Autosubst.
+
+
+From MyProject.src.OSum Require Export OSum persistent_pred wp_rules.
+
+Definition specN := nroot .@ "spec".
+
+Definition D `{Σ : gFunctors}:= persistent_pred (val * val) (iProp Σ).
+
+Definition spec_thread : ucmra := gmapUR nat (exclR exprO).
+
+Definition configRA : cmra := prodUR spec_thread (gsetUR loc).
+
+Class configSpec Σ := CS { 
+    config_in :: inG Σ (authR configRA) ; 
+(*     spec_predicates :: savedPredG Σ (val * val) ;
+ *)    config_name : gname
+}.
+
+Check authR.
+Section definitionsS.
+    Context `{configSpec Σ, invGS Σ}.
+
+    Definition spec_inv (e : expr)(s : state) : iProp Σ := 
+        (∃ e' s', own config_name (● ({[ 0 := Excl e']} , (list_to_set s')))
+                    ∗ ⌜rtc erased_step ([e],s) ([e'],s')⌝)%I.
+
+    Definition spec_ctx : iProp Σ :=
+        (∃ e s, inv specN (spec_inv e s))%I.
+
+    Definition tpool_pointsto (e : expr) : iProp Σ :=
+        own config_name (◯ ({[ 0 := Excl e ]}, ∅)).
+    
+    Definition spec_state_elem (l : loc) : iProp Σ :=
+        own config_name (◯ (empty, {[ l ]})).
+
+    Global Instance spec_ctx_persistent : Persistent spec_ctx.
+    Proof. apply _. Qed.
+
+End definitionsS.
+
+Notation "⤇ e" := (tpool_pointsto e) (at level 20) : bi_scope.
+Notation "l ∈s" := (spec_state_elem  l) (at level 20) : bi_scope.
+
+
+Section cfg.
+    Context `{ invGS Σ , configSpec Σ}.
+
+    Lemma step_pure' E  K e e' (P : Prop) n :
+        P →
+        PureExec P n e e' →
+        nclose specN ⊆ E →
+        spec_ctx ∗ (⤇ fill K e) ={E}=∗ (⤇ fill K e').
+    Proof.
+        iIntros (HP Hexe ?) "[#Hinv He]".
+        rewrite /spec_ctx /tpool_pointsto.
+        iDestruct "Hinv" as (ei si) "Hspec".
+        iInv specN as ">[%ei' [%si' [Hown %Hrtc]]]".
+        (* two assignments to own config_name *)
+        Check prod_included.
+        iCombine "Hown He" gives "%fo".
+    Admitted.
+
+    Lemma do_step_pure E  K e e' `{!PureExec True 1 e e'}:
+        nclose specN ⊆ E →
+        spec_ctx ∗ ⤇ fill K e ={E}=∗ ⤇ fill K e'.
+    Proof. by eapply step_pure'; last eauto. Qed.
+    
+    Lemma step_fst E  K e1 v1 e2 v2 :
+        to_val e1 = Some v1 → 
+        to_val e2 = Some v2 → 
+        nclose specN ⊆ E →
+        spec_ctx ∗ ⤇ fill K (Fst (Pair e1 e2)) ={E}=∗ ⤇ fill K e1.
+    Proof. by intros; apply: do_step_pure. Qed.
+
+    Lemma step_snd E  K e1 v1 e2 v2 :
+        to_val e1 = Some v1 → 
+        to_val e2 = Some v2 → 
+        nclose specN ⊆ E →
+        spec_ctx ∗ ⤇ fill K (Snd (Pair e1 e2)) ={E}=∗ ⤇ fill K e2.
+    Proof. by intros; apply: do_step_pure. Qed.
+
+    Lemma step_caseOf_true E K l e2 e3 e4 v2: 
+        to_val e2 = Some v2 →
+        nclose specN ⊆ E →
+        spec_ctx ∗ ⤇ fill K (CaseOf (Inj (Case l) e2) (Case l) e3 e4)  ={E}=∗ ⤇ fill K e3.[e2/].
+    Proof.
+        intros. apply do_step_pure.
+        -  apply wp_case_match. exists v2. apply of_to_val. done.
+        - done.
+    Qed. 
+
+    Lemma step_caseOf_false E K l l' e2 e3 e4 v2: 
+        to_val e2 = Some v2 →
+        nclose specN ⊆ E →
+        l <> l' →
+        spec_ctx ∗ ⤇ fill K (CaseOf (Inj (Case l) e2) (Case l') e3 e4)  ={E}=∗ ⤇ fill K e4.
+    Proof.
+        intros. apply do_step_pure.
+        -  apply wp_case_nomatch. exists v2. apply of_to_val; done. done.
+        -done.
+    Qed. 
+
+End cfg.
+
+
+
+        (* 
+    
+
+(* need to enhance state.. *)
+Class logrelSig  Σ := Resources {
+    invariants : invGS Σ;
+    predicates :: savedPredG Σ (val * val) ;
+    names :: gset_bijG Σ loc loc ;
+    name_set : gname
+}.
+Check rtc.
+Check erased_step. 
+Locate erased_step.
+Check gset_bijR.
+
+Check authR.
+Definition combine (l1 l2 : list loc) : gset (loc * loc) := 
+    list_to_set (zip l1 l2).
+
+(* not sure about the camera for the expression ..
+   want a unital camera    *)
+Definition spec_thread : cmra := exclR exprO.
+(* Definition tpoolUR : ucmra := gmapUR nat (exclR exprO).
+ *)
+
+ (* The data for our ghost execution
+ it is the program itself and a bijection of locations it maintains as program state? *)
+ Definition configRA : cmra := prodR spec_thread (gset_bijR loc loc).
+
+Definition as_thread (e : expr) : spec_thread := Excl e.
+
+Class configSpec Σ := CS { 
+    config_in :: inG Σ configRA ; 
+    spec_predicates :: savedPredG Σ (val * val) ;
+    config_name : gname
+}.
+
+Section definitionsS.
+    Context `{configSpec Σ, invGS Σ}.
+    (* This is similar to the state interpretation in the unary relation
+     
+    For some expression e in program state s,
+        There exists some (e',s') with logical state s'log reachable from (e,s)
+        such that
+            there is a bijection between s' and s'log in the ghost state
+            and for every l in s'log, there is a value predicate
+
+    wait.. shouldn't the ghost state now have value relations?
+        or is that SystemG.. 
+    *)
+    Definition spec_inv (e : expr)(s : state) : iProp Σ := 
+        (∃ e' s' s'log, own config_name (Excl e' , ●V (combine s' s'log))
+                    ∗ [∗ list] l' ∈ s'log, (∃ (P : D), saved_pred_own l' (DfracDiscarded) P)
+                    ∗ ⌜rtc erased_step ([e],s) ([e'],s')⌝)%I.
+
+    Definition spec_ctx : iProp Σ :=
+        (∃ e s, inv specN (spec_inv e s))%I.
+
+    Definition spec_points_to_pred (l' : loc)(P : @D Σ) : iProp Σ := 
+        (∃ e l, 
+            own config_name (Excl e, ◯V {[ (l, l') ]}) ∗
+            saved_pred_own l' (DfracDiscarded) P)%I.
+
+    Definition spec_pointer (e : expr) : iProp Σ := 
+        own config_name (Excl e , ◯V empty).
+
+End definitionsS.
+
+Notation "l ↦ₛ P" := (spec_points_to_pred l P) (at level 20) : bi_scope.
+Notation "⤇ e" := (spec_pointer e) (at level 20) : bi_scope.
+
+Section cfg.
+    Context `{logrelSig Σ, invGS Σ , configSpec Σ}.
+
+    Check specN.
+    Check fupd.
+    Print coPset.
+    Search coPset.
+    Check nclose specN.
+    Print UpClose.
+    
+    (* opening invariants  *)
+    Lemma inv_open_fail  (N : namespace) (P Q : iProp Σ) :
+        inv N (P) ⊢ Q.
+    Proof.
+        iIntros "Hinv".
+        Fail iInv "Hinv" as "HP".
+    Abort.
+
+    Lemma inv_open_fail (N : namespace) (P Q : iProp Σ) `{!Persistent P}  :
+        inv specN (P) ∗ (P -∗ Q)⊢ |={nclose specN}=> Q.
+    Proof.
+        iIntros "(Hinv & HPQ)".
+        iInv "Hinv" as "#HP".
+        iModIntro.
+        iSplit. 
+        - iApply "HP".
+        - iModIntro. iApply "HPQ".  iLöb as "H".
+    Abort.
+
+    Lemma step_pure' E  K e e' (P : Prop) n :
+        P →
+        PureExec P n e e' →
+        nclose specN ⊆ E →
+        spec_ctx ∗ ⤇ fill K e ={E}=∗ ⤇ fill K e'.
+    Proof.
+        iIntros (HP Hexe ?) "[#Hinv He]".
+        iDestruct "Hinv" as (ei si) "Hspec".
+        iInv 
+        iInv specN as (a b c) ">d" .
+
+
+
+
+Definition state_interp `{logrelSig Σ} (s : list loc) : iProp Σ :=
+    ∃ (s' : list loc ) , 
+            gset_bij_own_auth name_set (DfracOwn 1) (combine s s')  ∗
+            [∗ list] l' ∈ s', (∃ (P : D), saved_pred_own l' (DfracDiscarded) P).
+
+
+Global Instance OSum_irisGS `{logrelSig Σ} : irisGS OSum_lang Σ := {
+    iris_invGS := invariants;
+    num_laters_per_step _ := 0;
+    state_interp s  _ _ _ := state_interp s;
+    fork_post _ := True%I;
+    state_interp_mono _ _ _ _ := fupd_intro _ _
+}.
+ *)
